ver2/symbolic_execution.v
@@ -1,5 +1,6 @@
 Require Import bbv.Word.
 Require Import Nat.
+Require Import Coq.NArith.NArith.
 
 Require Import FORVES.constants.
 Import Constants.
@@ -29,6 +30,18 @@ Definition push_s (value : EVMWord) :=
     match push (Val value) sstk with
     | None => None
     | Some sstk' => Some (set_stack_sst sst sstk')
+    end.
+
+Definition pushtag_s (value : N) :=
+  fun (sst : sstate) (ops: stack_op_instr_map) =>
+    let sstk := get_stack_sst sst in
+    let sm : smap := get_smap_sst sst in
+    let v : smap_value := SymPUSHTAG value in
+    match add_to_smap sm v with
+    | pair key sm' =>
+        let sst' := set_stack_sst sst ((FreshVar key)::sstk) in
+        let sst'' := set_smap_sst sst' sm' in
+        Some sst''
     end.
 
 Definition pop_s (sst : sstate)  (ops: stack_op_instr_map) : option sstate :=
@@ -149,6 +162,7 @@ Definition exec_stack_op_intsr_s (label : stack_op_instr) (sst : sstate) (ops : 
 Definition evm_exec_instr_s (inst: instr) (sst: sstate) (ops: stack_op_instr_map) : option sstate :=
   match inst with
   | PUSH size w => (push_s (NToWord EVMWordSize w)) sst ops
+  | PUSHTAG v => (pushtag_s v) sst ops
   | POP => pop_s sst ops
   | DUP pos => dup_s pos sst ops
   | SWAP pos => swap_s pos sst ops
