ver2/symbolic_state_eval.v
@@ -60,6 +60,10 @@ Fixpoint eval_sstack_val (sv : sstack_val) (stk : stack) (mem: memory) (strg: st
             (* basic value: we just evaluate 'v' recursively, it is a stack element *)
             | SymBasicVal v => eval_sstack_val v stk mem strg ctx sb' ops
 
+            (* PUSHTAG *)
+            | SymPUSHTAG v =>
+                let tags := (get_tags_ctx ctx) in Some (tags v)
+                                               
             (* stack operation instruction: we evaluate the argument
             recursively and then evaluate the corresponding operation *)
             | SymOp label args =>
